theories/run_prop_hard.v
@@ -5,7 +5,7 @@ From det Require Import zify_ssreflect.
 Section s.
   Variable u : Unif.
 
-  Lemma next_alt_exp_same {s A r}:
+  (* Lemma next_alt_exp_same {s A r}:
     expand u s A = r -> is_fail r = false -> is_solved r = false ->
       next_alt false A = Some A.
   Proof.
@@ -23,6 +23,69 @@ Section s.
       rewrite sA success_failed//.
       have:= HB (get_substS s A').
       case Y: expand => //=[s'' B'|s'' B'] /(_ erefl erefl) ->//.
+  Qed. *)
+
+
+  Lemma runb_success1 {A} s: 
+    success A -> runb u s A (Some (get_substS s A)) (build_na A (next_alt true A)) 0.
+  Proof.
+    move=> sA.
+    apply: run_done.
+    apply: succes_is_solved sA.
+    move=> //.
+  Qed.
+
+  Lemma runb_success {A s1 s2 r n}: 
+    success A -> runb u s1 A s2 r n -> (s2 = Some (get_substS s1 A) /\ r = build_na A (next_alt true A) /\ n = 0)%type2.
+  Proof.
+    move=> sA H; have:= succes_is_solved u s1 sA.
+    inversion H; clear H; try congruence; subst.
+    - by rewrite H0 => -[??]; subst.
+    - by rewrite failed_success in sA.
+    - by rewrite failed_success in sA.
+  Qed.
+
+  Lemma run_consistent {s A s1 B s2 C n1 n2}:
+    runb u s A s1 B n1 -> runb u s A s2 C n2 -> ((s2 = s1) /\ (C = B) /\ (n2 = n1))%type2.
+  Proof.
+    move=> H; elim: H s2 C n2; clear.
+    + move=> s1 s2 r A B HA ? s3 C n2 H; subst.
+      have [[??]sA]:= expand_solved_same _ HA; subst.
+      by apply: runb_success sA H.
+    + move=> s1 s2 s3 r n1 A B HA HB IH s4 r' n2 H.
+      inversion H; clear H; try congruence; subst.
+      - move: H0; rewrite HA => -[??]; subst; by rewrite !(IH _ _ _ H1)//.
+      - by rewrite failed_expand in HA.
+      - by rewrite failed_expand in HA.
+    + move=> s1 s2 s3 r n1 A B HA HB IH s4 r' n2 H.
+      inversion H; clear H; try congruence; subst.
+      - move: H0; rewrite HA => -[??]; subst; by rewrite !(IH _ _ _ H1)//.
+      - by rewrite failed_expand in HA.
+      - by rewrite failed_expand in HA.
+    + move=> s1 s2 A B r n1 fA nB rB IH s3 C n2 H.
+      inversion H; clear H; try congruence; subst; try by rewrite failed_expand in H0.
+      move: H1; rewrite nB => -[?]; subst.
+      by apply: IH.
+    + move=> s1 A fA nA s2 C n2 H.
+      inversion H; subst; try congruence; try rewrite //failed_expand// in H0.
+  Qed.
+
+  Lemma is_ko_runb {s A}: is_ko A -> runb u s A None (dead1 A) 0.
+  Proof.
+    elim: A s => //=.
+    - by move=> s _; apply: run_dead => //=.
+    - move=> s _; apply: run_dead => //=.
+    - move=> A HA s B HB s2 /andP[kA kB].
+      have {}HA := HA s2 kA.
+      have {}HB := HB s2 kB.
+      apply: run_dead; rewrite/=.
+        by rewrite !is_ko_failed//if_same.
+      by rewrite !is_ko_next_alt// !if_same.
+    - move=> A HA B0 HB0 B HB s kA.
+      have {HB}HA := HA s kA.
+      apply: run_dead => /=.
+        by rewrite is_ko_failed.
+      by rewrite (is_ko_next_alt _ kA)// is_ko_failed//=if_same.
   Qed.
 
   Lemma runb_or0 {s1 A s B s2 r b}:
@@ -36,207 +99,275 @@ Section s.
       case: ifP => dC.
         case X: expand => //[s' D'|s' D'][??]; subst; by apply: IH.
       case Y: expand=> //[s1' C'|s1' C'][??]; subst; by apply: IH.
-    - move=> s1 s2 A B C r n /expand_failed_same [? _] + _ IH D s3 E ?; subst => /=.
-      case: ifP => //dD.
-        by case: next_alt => //? [?]; subst; apply: IH.
-      case: next_alt => //. 
-        by move=> ?[?]; subst; apply: IH.
+    - move=> s1 s2 A B r n _ + H IH C s3 D ?; subst => /=.
+      case: ifP => //= _.
+        case: next_alt => //= ? [/esym]; apply IH.
+      case: next_alt => //=.
+        move=>? [/esym]; apply IH.
       case: ifP => // _.
-      case: next_alt => //. 
-      by move=> ?[?]; subst; apply: IH.
+      case: next_alt => //= ? [/esym]; apply IH.
+  Qed.
+
+  Lemma next_alt_not_failed A:
+    (failed A) = false -> next_alt false A = Some A.
+  Proof.
+    elim: A => //=.
+    - move=> A HA s B HB; case: ifP => dA fB.
+        rewrite HB//=.
+      rewrite HA//.
+    - move=> A HA B0 _ B HB.
+      case: ifP => dA.
+        rewrite is_dead_failed//.
+      case: ifP => //=fA.
+      case: ifP => //=sA fB.
+      rewrite HB//.
   Qed.
 
   Lemma next_alt_runb {A B C s s2 b1}:
-    next_alt false A = Some B ->
-      runb u s B s2 C b1 ->
+    next_alt false A = B ->
+      runb u s (build_na A B) s2 C b1 ->
         runb u s A s2 C b1.
   Proof.
+    move=> <-{B}.
     case fA: (failed A).
-      repeat eexists; apply: run_fail; eauto.
-      by apply: failed_expand.
-    by rewrite next_alt_not_failed// => -[->].  
+      case X: next_alt => [A'|]/= H.
+        apply: run_fail fA X H.
+      have [->[->->]]:= run_dead2 _ H.
+      apply: run_dead fA X.
+    rewrite next_alt_not_failed//.
   Qed.
 
-  Lemma run_ko_left1 {s1 s2 A B b sx r}:
-    is_ko A -> runb u s1 (Or A s2 B) sx r b ->
-      Texists b r', runb u s2 B sx r' b /\ 
-        (omap (fun x => Or (if is_dead A then A else dead1 A) s2 x) r' = r).
-  Proof.
-    remember (Or A _ _) as o1 eqn:Ho1 => + H.
-    elim: H A B s2 Ho1; clear.
-    + move=> s s' r A B H ->  A' B' s2 ? kA'; subst.
-      have [[??]sA]:= expand_solved_same _ H; subst.
-      move: sA => /=.
-      case: ifP => [dA sB|dA sA]; last first.
-        by rewrite is_ko_success in sA.
-      repeat eexists; auto.
-      apply: run_done (succes_is_solved _ _ sB) erefl.
-    - move=> s1 s2 s3 r A B n + HB IH C D s4 ? kC; subst => /=.
-      case: ifP => dC; case X: expand => //.
-    - move=> s1 s2 s3 r A B n + HB IH C D s4 ? kC; subst => /=.
-      case: ifP => dC.
-        case X: expand => //[s4' D'|s4' D'][??]; subst; 
-        have {IH} [b[r'[H1 H2]]]:= IH _ _ _ erefl kC; subst; rewrite dC in HB; subst;
-        rewrite dC; repeat eexists.
-          apply:run_step X H1.
-        apply:run_cut X H1.
-      by rewrite is_ko_expand.
-    - move=> s1 s2 A B C r n /expand_failed_same [? +] + rC IH D E s3 ? kD; subst.
-      rewrite /=(is_ko_next_alt _ kD).
-      case: ifP => [dD fE|dD fD].
-        case X: next_alt => //[E'][?]; subst.
-        have [b[r'[{}IH H]]] := IH _ _ _ erefl kD; subst; rewrite dD/= in rC; subst.
-        rewrite dD; repeat eexists.
-        apply: run_fail; eauto.
-        by apply: failed_expand.
-      case: ifP => //dE.
-      case W: next_alt => //[E'][?]; subst.
-      have [b[r'[{}IH H]]] := IH _ _ _ erefl (is_dead_is_ko is_dead_dead).
-      rewrite is_dead_dead/= in H; subst.
-      have {W IH} := next_alt_runb W IH.
-      repeat eexists; eauto.
-  Qed.
+  Definition get_dead A B := if is_dead A && ~~(is_dead B) then A else dead1 A.
 
-  Lemma run_ko_left2 {s2 X B r SOL b1} sIgn:
-    is_ko X -> runb u s2 B SOL r b1 ->
-    runb u sIgn (Or X s2 B) SOL (omap (fun x => Or (if is_dead X then X else dead1 X) s2 x) r) 0.
+  Lemma run_ko_left1 {s1 s2 A B A' B' sx}:
+    is_ko A -> runb u s1 (Or A s2 B) sx (Or A' s2 B') 0 ->
+      Texists b, runb u s2 B sx B' b /\ 
+        (A' = get_dead A B').
   Proof.
-    move=> + HB; elim: HB sIgn X; clear.
-    + move=> s s' r A B /expand_solved_same [[??]sB] ? sIgn X kX; subst => /=.
-      case dX: (is_dead X).
+    rewrite/get_dead.
+    remember (Or A _ _) as o1 eqn:Ho1.
+    remember (Or A' _ _) as o2 eqn:Ho2 => + H.
+    elim: H A B A' B' s2 Ho1 Ho2; clear.
+    + move=> s s' A B _ + <-  A1 B1 A2 B2 s2 ? + kA'; subst.
+      move=> /expand_solved_same [[??]+]; subst => /=.
+      rewrite (is_ko_success kA') (is_ko_next_alt _ kA').
+      case: ifP =>// dA1 sB1.
+      case X: next_alt => //=[B1'|] [??]; subst.
         repeat eexists.
           apply: run_done.
-            rewrite/= (succes_is_solved _ _ sB) is_ko_expand// .
-          rewrite dX => //.
-        by move=> /=; rewrite dX/=; case: next_alt; auto.
+            apply: succes_is_solved sB1.
+          by rewrite X.
+        rewrite (next_alt_dead X)//.
       repeat eexists.
+      apply: run_done.
+        apply: succes_is_solved sB1.
+        rewrite X => //.
+      rewrite is_dead_dead//.
+    - move=> s1 s2 s3 r A B n + HB IH A1 A2 B1 B2 s4 ?? kA1; subst => /=.
+      case: ifP => dC; case X: expand => //.
+    - move=> s1 s2 s3 r A B n + HB IH A1 A2 B1 B2 s4 ?? kA1; subst => /=.
+      rewrite (is_ko_expand _ kA1)//.
+      case: ifP => dC//.
+      case X: expand => //[s4' D'|s4' D'][??]; subst;
+      have {IH} [b[H1 ?]] := IH _ _ _ _ _ erefl erefl kA1; subst; rewrite dC/=;
+      repeat eexists.
+        apply:run_step X H1.
+      apply:run_cut X H1.
+    - move=> s1 s2 A B r n ++ rB IH A1 A2 B1 B2 s3 ?? kA1; subst => /=.
+      rewrite (is_ko_next_alt _ kA1).
+      case: ifP => /=dA H1.
+        case X: next_alt => [A2'|]//=.
+          move=> [?]; subst.
+          have [b[H3 H4]] := IH _ _ _ _ _ erefl erefl kA1; subst.
+          rewrite dA/=; repeat eexists.
+          apply: run_fail H1 X H3.
+        case: ifP => // dA2.
+        case X: next_alt => //[A2'][?]; subst.
+        have [b[H3]]:= IH _ _ _ _ _ erefl erefl (is_dead_is_ko is_dead_dead).
+        rewrite is_dead_dead dead2 if_same => ?; subst.
+        repeat eexists.
+        apply: next_alt_runb X H3.
+    - move=> _ A + + B1 C1 B2 C2 s ?/= + kB1; subst => /=++[??]; subst.
+      rewrite (is_ko_next_alt _ kB1).
+      rewrite is_dead_dead /= andbF.
+      case: ifP => dB1 F.
+        case X: next_alt => [C1'|]// _.
+        repeat eexists; apply: run_dead F X.
+      case: ifP => dC1.
+        repeat eexists; apply: run_dead.
+          apply: is_dead_failed dC1.
+        rewrite is_dead_next_alt//.
+      case X: next_alt => // _.
+      repeat eexists.
+      case fC1: (failed C1).
+        apply: run_dead fC1 X.
+      by rewrite next_alt_not_failed in X.
+  Qed.
+
+  Lemma run_ko_left2 {s2 X B B' r b1} sIgn:
+    is_ko X -> runb u s2 B r B' b1 ->
+    runb u sIgn (Or X s2 B) r (Or (get_dead X B') s2 B') 0.
+  Proof.
+    rewrite/get_dead.
+    move=> + HB; elim: HB sIgn X; clear.
+    + move=> s s' r A B /expand_solved_same [[??]sB] ? sIgn X kX; subst => /=.
+      case dX: (is_dead X) => /=.
+        apply: run_done.
+          by rewrite/= (succes_is_solved _ _ sB) is_ko_expand// dX.
+        rewrite/=dX; case Y: next_alt => //=[A'|].
+          by rewrite (next_alt_dead Y)//.
+        by rewrite is_dead_dead//.
       apply: run_fail => /=.
-        by rewrite dX is_ko_expand//.
+        by rewrite dX is_ko_failed.
         by rewrite/= dX is_ko_next_alt// success_is_dead// next_alt_not_failed// success_failed//.
       apply: run_done.
         rewrite/= (succes_is_solved _ _ sB) is_dead_dead//.
-      rewrite /=is_dead_dead//.
+      by rewrite /=is_dead_dead//; case: next_alt => //=; rewrite dead2//.
     + move=> s1 s2 s3 r A B n HA HB IH sIgn X kX.
-      case dX: (is_dead X).
+      case dX: (is_dead X) => /=.
         have {}IH := IH sIgn _ kX.
         rewrite dX in IH.
-        apply: run_step.
-          rewrite /= dX HA//.
-        by eassumption.
+        apply: run_step IH.
+        by rewrite /= dX HA//.
       have {}IH:= IH sIgn (dead1 X) (is_dead_is_ko is_dead_dead).
-      rewrite is_dead_dead in IH.
-      repeat eexists.
+      rewrite is_dead_dead dead2 if_same in IH.
+      have fA := expand_not_failed _ HA notF.
       apply: run_fail.
-        rewrite/=dX is_ko_expand//.
-        move=>/=; rewrite dX is_ko_next_alt//.
-        have fA := expand_not_failed _ HA notF.
-        rewrite next_alt_not_failed//failed_dead//.
+        rewrite/=dX is_ko_failed//.
+        by rewrite /= dX is_ko_next_alt// next_alt_not_failed//=failed_dead.
       apply: run_step IH.
       rewrite /=is_dead_dead HA//.
     (* TODO: the following case is same as previous... *)
     + move=> s1 s2 s3 r A B n HA HB IH sIgn X kX.
-      case dX: (is_dead X).
+      case dX: (is_dead X) => /=.
         have {}IH := IH sIgn _ kX.
         rewrite dX in IH.
-        apply: run_step.
-          rewrite /= dX HA//.
-        by eassumption.
+        apply: run_step IH.
+        by rewrite /= dX HA//.
       have {}IH:= IH sIgn (dead1 X) (is_dead_is_ko is_dead_dead).
-      rewrite is_dead_dead in IH.
-      repeat eexists.
+      rewrite is_dead_dead dead2 if_same in IH.
+      have fA := expand_not_failed _ HA notF.
       apply: run_fail.
-        rewrite/=dX is_ko_expand//.
-        move=>/=; rewrite dX is_ko_next_alt//.
-        have fA := expand_not_failed _ HA notF.
-        rewrite next_alt_not_failed//failed_dead//.
+        rewrite/=dX is_ko_failed//.
+        by rewrite /= dX is_ko_next_alt// next_alt_not_failed//=failed_dead.
       apply: run_step IH.
       rewrite /=is_dead_dead HA//.
-    + move=> s1 s2 A B C r n /expand_failed_same [? fB] nB rC IH sIgn X kX; subst.
+    + move=> s1 s2 A B r n fA nB rC IH sIgn X kX; subst.
       case dX: (is_dead X).
         have {}IH:= IH sIgn _ kX.
-        rewrite dX in IH; subst.
-        repeat eexists.
-        apply: run_fail IH.
-          rewrite/= dX failed_expand//.
-        rewrite/= dX nB//.
+        rewrite dX/= in IH; subst.
+        by apply: run_fail IH; rewrite /=dX//nB//.
       have {}IH:= IH sIgn (dead1 X) (is_dead_is_ko is_dead_dead).
-      rewrite is_dead_dead in IH; subst.
-      repeat eexists; repeat eexists.
-      apply: run_fail IH.
-        rewrite/=dX is_ko_expand//.
-      move=>/=; rewrite dX is_ko_next_alt//(next_alt_dead nB) nB//.
+      rewrite is_dead_dead/=dead2 if_same in IH; subst.
+      apply: run_fail IH; rewrite/= dX ?is_ko_failed// is_ko_next_alt//nB.
+      rewrite (next_alt_dead nB)//.
+    + move=> s1 B fB nB sIgn X kX.
+      rewrite is_dead_dead andbF.
+      apply: run_dead; rewrite/=.
+        by rewrite fB is_ko_failed//if_same.
+      by rewrite nB is_ko_next_alt// !if_same.
   Qed.
 
   Lemma run_or_ko_right1 {s2 X B B' SOL b1} sIgn:
     is_ko X -> runb u s2 B SOL B' b1 ->
-    runb u s2 (Or B sIgn X) SOL (omap (fun x => Or x sIgn (if b1 == 0 then X else cutr X)) B') 0.
+    runb u s2 (Or B sIgn X) SOL (Or B' sIgn (if is_dead B' then dead1 X else if b1 == 0 then X else cutr X)) 0.
   Proof.
     move=> + HB; elim: HB sIgn X; clear.
     + move=> s s' r A B /expand_solved_same [[??]sB] ? sIgn X kX; subst => /=.
       apply: run_done.
-        rewrite/= success_is_dead// succes_is_solved//.
+        by rewrite/= success_is_dead// succes_is_solved//.
       rewrite/= success_is_dead// (is_ko_next_alt _ kX)// if_same//.
+      case W: next_alt => //=[A'|].
+        rewrite (next_alt_dead W)//.
+      rewrite is_dead_dead//.
     + move=> s1 s2 s3 r A B n HA HB IH sIgn X kX.
       apply: run_step.
         by rewrite/= HA; case: ifP => //dA; rewrite is_dead_expand in HA.
       have:= IH sIgn (cutr X) is_ko_cutr.
-      by rewrite cutr2 if_same.
+      rewrite cutr2 if_same dead_cutr//.
     + move=> s1 s2 s3 r A B n HA HB IH sIgn X kX.
       apply: run_step.
-        by rewrite/=HA; case: ifP => //dA; rewrite is_dead_expand in HA.
-      by apply: IH.
-    + move=> s1 s2 A B C r n /expand_failed_same [? fB] nB rC IH sIgn X kX; subst.
-      apply: run_fail.
-        rewrite/= (failed_expand _ fB)//; rewrite (next_alt_dead nB)//.
-        move=>/=; rewrite (next_alt_dead nB) nB//.
-      by apply: IH.
+        by rewrite/= HA; case: ifP => //dA; rewrite is_dead_expand in HA.
+      apply: IH => //.
+    + move=> s1 s2 A B r n fA nA rB IH sIgn X kX.
+      apply: run_fail => /=.
+        by rewrite fA is_ko_failed//if_same.
+      rewrite (is_ko_next_alt _ kX) nA (next_alt_dead nA)//.
+      apply: IH kX.
+    + move=> s1 A fA nA sIgn X kX.
+      rewrite is_dead_dead.
+      apply: run_dead => /=.
+        by rewrite fA is_ko_failed// if_same.
+      by rewrite is_ko_next_alt//nA !if_same.
   Qed.
 
-  Lemma run_or_ko_right2 {s2 X B SOL r sIgn b}:
-    is_ko X -> runb u s2 (Or B sIgn X) SOL r b ->
-      Texists b1 r', runb u s2 B SOL r' b1 /\ omap (fun x => Or x sIgn (if b1 == 0 then X else cutr X)) r' = r.
+  Lemma run_or_ko_right2 {s2 X X' A A' SOL sIgn}:
+    is_ko X -> runb u s2 (Or A sIgn X) SOL (Or A' sIgn X') 0 ->
+      Texists b1, runb u s2 A SOL A' b1 /\ X' = if is_dead A' then dead1 X else if b1 == 0 then X else cutr X.
   Proof.
-    remember (Or _ _ _) as o eqn:Ho => +HB.
-    elim: HB B sIgn X Ho; clear.
-    + move=> s s' r A B /expand_solved_same [[??]+] ? C sIgn X ? kX; subst => /=.
-      rewrite is_ko_success//.
-      case: ifP => //dC sC.
-      rewrite (is_ko_next_alt _ kX) if_same.
+    remember (Or A _ _) as o1 eqn:Ho1.
+    remember (Or A' _ _) as o2 eqn:Ho2 => + H.
+    elim: H A X A' X' Ho1 Ho2; clear.
+    + move=> s s' A B _ + <-  A1 B1 A2 B2 ? + kB'; subst.
+      move=> /expand_solved_same [[??]+]; subst => /=.
+      rewrite (is_ko_success kB') (is_ko_next_alt _ kB').
+      case: ifP =>// dA1 sB1.
+      rewrite (is_ko_next_alt _ kB') if_same.
+      case X: next_alt => //=[B1'|][??]; subst.
+        repeat eexists.
+          apply: run_done.
+            apply: succes_is_solved sB1.
+          by rewrite X.
+        by rewrite (next_alt_dead X)//.
       repeat eexists.
-      apply: run_done (succes_is_solved _ _ sC) erefl.
-      by auto.
-    + move=> s1 s2 s3 r A B n + HB IH C sIgn X ? kX; subst => /=.
-      case: ifP; case: expand => //.
-    + move=> s1 s2 s3 r A B n + HB IH C sIgn X ? kX; subst => /=.
-      rewrite (is_ko_expand _ kX); case: ifP => //dC.
-      case W: expand => //[s1' C'|s1' C'][??]; subst.
-        have [b1[r' [{}IH H]]] := IH _ _ _ erefl kX; subst.
-        repeat eexists; apply: run_step W IH.
-      have [b1[r' [{}IH H]]] := IH _ _ _ erefl is_ko_cutr; subst.
+      apply: run_done.
+        apply: succes_is_solved sB1.
+        rewrite X => //.
+      rewrite is_dead_dead//.
+    - move=> s1 s2 s3 r A B n + HB IH A1 A2 B1 B2 ?? kA1; subst => /=.
+      case: ifP => dC; case X: expand => //.
+    - move=> s1 s2 s3 r A B n + HB IH A1 A2 B1 B2 ?? kA1; subst => /=.
+      rewrite (is_ko_expand _ kA1)//=.
+      case: ifP => dC//.
+      case X: expand => //[s4' D'|s4' D'][??]; subst;
+      have := IH _ _ _ _ erefl erefl.
+        move=> /(_ kA1) [b [{}IH ?]]; subst.
+        repeat eexists.
+        apply: run_step X IH.
+      move=> /(_ is_ko_cutr)[b [{}IH ?]]; subst.
+        repeat eexists.
+        apply: run_cut X IH.
+      rewrite cutr2 if_same dead_cutr.
+      by rewrite (runb_or0 HB)//.
+    - move=> s1 s2 A B r n ++ rB IH A1 A2 B1 B2 ?? kA1; subst => /=.
+      rewrite (is_ko_next_alt _ kA1) if_same.
+      case: ifP => //=dA H1.
+      case X: next_alt => [A2'|]//=[?]; subst.
+      have [b[{}IH ?]] := IH _ _ _ _ erefl erefl kA1; subst.
+      repeat eexists; apply: run_fail H1 X IH.
+    - move=> s1 ? ++ A X A' X' ? + kX; subst => /= ++[??]; subst.
+      rewrite is_ko_failed// is_ko_next_alt//= if_same is_dead_dead.
+      case: ifP => //=H1.
+        move=> _ _; repeat eexists.
+        apply: run_dead.
+          rewrite is_dead_failed//.
+        rewrite is_dead_next_alt//.
+      move=> fA; case W: next_alt => //= _.
       repeat eexists.
-        apply: run_cut W IH.
-      by rewrite cutr2 if_same.
-    + move=> s1 s2 A B C r n /expand_failed_same [? +] + rC IH D sIgn X ? kX; subst => /=.
-      rewrite (is_ko_next_alt _ kX) if_same.
-      case: ifP => //[dD fD].
-      case W: next_alt => //[D'][?]; subst.
-      have [b1[r' [{}IH H]]] := IH _ _ _ erefl kX; subst.
-      repeat eexists.
-      apply: next_alt_runb W IH.
+      apply: run_dead fA W.
   Qed.
 
-  Definition build_or_state cn sR R r rOR :=
-    if cn == 0 then
-      if r is Some A' 
-        then (rOR = (Some (Or A' sR R))) :> Type
-      else if next_alt false R is Some R' 
-        then Texists A'', is_dead A'' /\ (rOR = Some (Or A'' sR R'))
-      else rOR = None
-    else rOR = omap (fun x => Or x sR (cutr R)) r.
+  Definition build_or_state cn A' X :=
+    if cn == 0 then 
+      if is_dead A' then 
+        if next_alt false X is Some X' then X'
+        else dead1 X
+      else X
+    else if is_dead A' then dead1 X else cutr X.
 
-  Lemma build_or_state_inj {cn sR R r rOR} rOR1:
-    build_or_state cn sR R r rOR ->
-      build_or_state cn sR R r rOR1 -> rOR = rOR1.
+  (* Lemma build_or_state_inj {cn A A1} A2:
+    build_or_state cn A A1 ->
+      build_or_state cn A A2 -> A1 = A2.
   Proof.
     rewrite/build_or_state.
     case: eqP => [?|???]; subst => //.
@@ -246,182 +377,182 @@ Section s.
        add the state in option None in runb *)
     move=> [A1 [dA1 ?]] [A2 [dA2 ?]]; subst.
     repeat f_equal.
-  Admitted.
+  Admitted. *)
 
-  Lemma run_or_correct_left {s1 A s2 b r} sX X:
-    runb u s1 A s2 r b ->
-      Texists r', 
-        runb u s1 (Or A sX X) s2 r' 0 /\
-          build_or_state b sX X r r'.
+  Lemma run_or_correct_left {s1 A A' s2 b}:
+    runb u s1 A s2 A' b -> forall sX X,
+        if s2 is None then A' = dead1 A'
+          (* forall X', runb u s1 (Or A sX X)  <-> runb  *)
+        else runb u s1 (Or A sX X) s2 (Or A' sX (build_or_state b A' X)) 0
+          .
   Proof.
     rewrite/build_or_state.
-    move=> H; elim: H X; clear.
-    + move=> s s' r A B /[dup] /(expand_solved_same) [[??]sA] H ? X; subst.
-      repeat eexists.
-        apply: run_done erefl; rewrite /= H success_is_dead//.
-      rewrite//= success_is_dead//.
-      case W: next_alt => //=.
-      case Z: next_alt => //=[C'|].
-        rewrite (next_alt_dead Z); repeat eexists; rewrite is_dead_dead//.
-      rewrite if_same//.
-    + move=> s1 s2 s3 r A B n HA HB IH X/=.
-      case: n HB IH => //=.
-        move=> + /(_ (cutr X)) [r'[{}H1]].
-        case: r => [B'|].
-          move=> HB?; subst.
-          repeat eexists => //.
-          apply: run_step.
-            by rewrite/=HA; case: ifP => //dA; rewrite is_dead_expand in HA.
-          by [].
-        rewrite (is_ko_next_alt _ is_ko_cutr) => H2 ?; subst.
-        repeat eexists => //.
-        apply: run_step.
-          by rewrite/=HA; case: ifP => //dA; rewrite is_dead_expand in HA.
-        by [].
-      move=> n + /(_ (cutr X)) [r'[{}H1]].
-      rewrite cutr2.
-      case: r => [B'|].
-      move=> HB?; subst.
-        repeat eexists => //.
-        apply: run_step.
-          by rewrite/=HA; case: ifP => //dA; rewrite is_dead_expand in HA.
-        by [].
-      move => H2 ?; subst.
-      repeat eexists => //.
-      apply: run_step.
-        by rewrite/=HA; case: ifP => //dA; rewrite is_dead_expand in HA.
-      by [].
-    + move=> s1 s2 s3 r A B n HA HB IH X/=.
-      case: n HB IH => //=.
-        move=> + /(_ X) [r'[{}H1]].
-        case: r => [B'|].
-          move=> HB?; subst.
-          repeat eexists => //.
-          apply: run_step.
-            by rewrite/=HA; case: ifP => //dA; rewrite is_dead_expand in HA.
-          by [].
-        case Y: next_alt => [X'|].
-          move=> HB [A'' [dA'' ?]]; subst.
-          repeat eexists; eauto.
-          apply: run_step; eauto; rewrite/= HA.
-          by case: ifP => // dA; rewrite is_dead_expand in HA.
-        move=> rB ?; subst.
-        repeat eexists => //.
-        apply: run_step.
-          by move=> /=; rewrite HA; case: ifP => //dA;rewrite is_dead_expand in HA.
-        by [].
-      move=> n + /(_ (X)) [r'[{}H1]].
-      case: r => [B'|].
-      move=> HB?; subst.
-        repeat eexists => //.
-        apply: run_step.
-          by rewrite/=HA; case: ifP => //dA; rewrite is_dead_expand in HA.
-        by [].
-      move => H2 ?; subst.
-      repeat eexists => //.
-      apply: run_step.
-        by rewrite/=HA; case: ifP => //dA; rewrite is_dead_expand in HA.
-      by [].
-    + move=> s1 s2 A B C r n HA HB HC + X.
-      move=> /(_ X)[r' [H1 H2]].
-      repeat eexists; try eassumption.
-      apply: run_fail H1.
-        move=> /=; rewrite HA; case: ifP => //dA.
-        move: HA; rewrite is_dead_expand// =>-[?]; subst.
-        by rewrite is_dead_next_alt in HB.
-      by rewrite/= HB (next_alt_dead HB).
+    move=> H; elim: H; clear => //.
+    + move=> s s' A B r /[dup] /(expand_solved_same) [[??]sA] eA nB sX X; subst => /=.
+      apply: run_done => //=.
+        by rewrite eA success_is_dead//=.
+      rewrite /= success_is_dead//=.
+      case W: next_alt => //=[B'|].
+        rewrite (next_alt_dead W)//=.
+      rewrite is_dead_dead.
+      case: ifP => dX.
+        rewrite is_dead_next_alt//.
+      case X: next_alt => //.
+    + move=> s1 s2 s3 r A B n HA _ + sX X/=.
+      move=> /(_ sX (cutr X)); rewrite next_alt_cutr dead_cutr cutr2 if_same.
+      case: s3 => //s3.
+      apply: run_step => /=.
+      rewrite HA.
+      case: ifP => //dA.
+      by rewrite is_dead_expand in HA.
+    + move=> s1 s2 s3 r A B n HA _ + sX X/=.
+      move=> /(_ sX X).
+      case: s3 => //s3.
+      apply: run_step => /=.
+      rewrite HA.
+      case: ifP => //dA.
+      by rewrite is_dead_expand in HA.
+    + move=> s1 s2 A B r n fA nA _ IH sX X.
+      case: s2 IH => //[s2|] IH; auto.
+      apply: run_fail; rewrite /=?(next_alt_dead nA)//.
+      rewrite nA//.
+    + by move=>*; rewrite dead2.
   Qed.
 
-  Lemma run_or_complete {s1 s2 A B s3 r b}:
+  Lemma run_or_complete {s1 s2 A B s3 A' B'}:
   (* TODO: be more precise on altAB *)
-    runb u s1 (Or A s2 B) s3 r b ->
-      (Texists n r', (
-        (runb u s1 A s3 r' n /\ build_or_state n s2 B r' r)%type2
+    runb u s1 (Or A s2 B) s3 (Or A' s2 B') 0 ->
+      (Texists n1, (
+        if s3 is None then
+          runb u s1 A None A' n1 /\ (if n1 == 0 then Texists n2, runb u s2 B None B' n2 else B' = dead1 B) /\ A' = dead1 A' /\ B' = dead1 B'
+        else
+          True)).
+        (* (runb u s1 A s3 r' n /\ build_or_state n s2 B r' r)%type2
          + 
-        (runb u s2 B s3 r' n))%type).
+        (runb u s2 B s3 r' n))%type). *)
   Proof.
-    rewrite/build_or_state.
-    remember (Or _ _ _) as O1 eqn:HO1 => H.
-    elim: H s2 A B HO1 => //=; clear.
-    + move=> s1 s2 r A B /expand_solved_same [[??] +] ? s3 C D ?; subst => /=.
-      case:ifP => [dC sD|dC sC]; repeat eexists.
-        right; apply: run_done erefl.
-        by apply: succes_is_solved sD.
-      left; repeat eexists.
-        apply: run_done erefl.
-        by apply: succes_is_solved.
-      case X: next_alt => //=.
-      case Y: next_alt => //[D'|]; rewrite?if_same//.
-      repeat eexists; last first.
-        rewrite (next_alt_dead Y)//.
-      by rewrite is_dead_dead.
-    + move=> s1 s2 s3 r A B n + HB IH s4 C D ?; subst => /=.
-      by case: ifP; case: expand => //.
-    + move=> s1 s2 s3 r A B n + HB IH s4 C D ?; subst => /=.
-      case: ifP => dC.
-        case X: expand => //[s4' D'|s4' D'][??]; subst.
-          have := IH _ _ _ erefl => -[aB[b1 [[{}IH H1]|{}IH]]].
-            by have:= is_dead_runb _ dC IH.
-          repeat eexists; right.
-          apply: run_step X IH.
-        have := IH _ _ _ erefl => -[aB[b1 [[{}IH H1]|{}IH]]].
-          by have:= is_dead_runb _ dC IH.
-        repeat eexists; right.
-        apply: run_cut X IH.
-      case X: expand => //[s4' D'|s4' D'][??]; subst.
-        have := IH _ _ _ erefl => -[aB[b1 [[{}IH H1]|{}IH]]].
-          repeat eexists; left; split; eauto.
-          apply: run_step X IH.
-        by repeat eexists; eauto.
-      have := IH _ _ _ erefl => -[aB[b1 [[{}IH H1]|{}IH]]].
-        repeat eexists; left; split; eauto.
-          apply: run_cut X IH.
-        move: H1.
-        move=> /=; rewrite cutr2 next_alt_cutr.
-        case: eqP => //=?; subst.
-        case: b1 IH => //=.
-      by have:= is_ko_runb _ is_ko_cutr IH.
-    + move=> s1 s2 A B C r n /expand_failed_same [? +] + rC IH s3 D E ?; subst => /=.
-      case: ifP => [dD fE|dD fD].
-        case X: next_alt => //[E'][?]; subst.
-        have := IH _ _ _ erefl=> -[aB[b1 [[{}IH H1]|{}IH]]].
-          by have:= is_dead_runb _ dD IH.
-        repeat eexists; right.
-        apply: run_fail; eauto.
-        by apply: failed_expand.
-      case X: next_alt => //[D'|].
-        move=>[?]; subst.
-        have := IH _ _ _ erefl => -[aB[b1 [[{}IH H1]|{}IH]]].
-          repeat eexists; left; split; eauto.
-          apply: run_fail; eauto.
-          by apply: failed_expand.
-        by repeat eexists; right; eauto.
-      case: ifP => // dE; case W: next_alt => //[E'][?]; subst.
-      have := IH _ _ _ erefl => -[aB[b1 [[{}IH H1]|{}IH]]].
-        by have:= is_dead_runb _ is_dead_dead IH.
-      repeat eexists; right.
-      apply: next_alt_runb W IH.
+    (* rewrite/build_or_state. *)
+    remember (Or A _ _) as o1 eqn:Ho1.
+    remember 0 as z eqn:Hz.
+    remember (Or A' _ _) as o2 eqn:Ho2 => H.
+    elim: H s2 A B A' B' Ho1 Ho2 Hz => //=; clear.
+    + move=> s1 s2 s3 r A B n + HB IH s4 A1 A2 B1 B2 ???; subst => //=.
+      case: ifP => dA1.
+        case X: expand => //[s4' B''|s4' B''][??]; subst; have {IH}[n1+] := IH _ _ _ _ _ erefl erefl erefl.
+          case: s3 HB => [s3|] HB//.
+          move=> [H1[+[H3 H4]]]; subst.
+          case:eqP => H5; subst.
+            move=> [n2 H5].
+            repeat eexists; eauto => /=.
+            repeat eexists.
+            apply: run_step X H5.
+          move=> ?; subst; rewrite dead2.
+          repeat eexists; eauto.
+          case: eqP => //.
+          by have [_[??]] := run_dead1 _ dA1 H1; subst.
+        case: s3 HB => [s3|] HB//.
+        move=> [H1[H2[H3 H4]]]; subst.
+        repeat eexists; eauto; move:H2; case:eqP => H; subst.
+          move=> [n2 H].
+          eexists; apply: run_cut X H.
+        move=> ?; subst.
+        by have [_[??]] := run_dead1 _ dA1 H1; subst.
+      case X: expand => //[s4' D'|s4' D'][??]; subst; have {IH}[n1] := IH _ _ _ _ _ erefl erefl erefl.
+        case: s3 HB => [s3|] HB//.
+        move=> [H1[H2[H3 H4]]]; subst.
+        repeat eexists; eauto.
+        apply: run_step X H1.
+      case: s3 HB => [s3|] HB//.
+      move=> [H1[H2[H3 H4]]]; subst.
+      move: H2; case:eqP => H; subst.
+        move=>[n2]/(run_consistent (is_ko_runb is_ko_cutr)) [?[??]]; subst.
+        rewrite dead2 dead_cutr.
+        repeat eexists; eauto.
+          apply: run_cut X H1.
+        by [].
+      move=> ?; subst.
+      rewrite dead2 dead_cutr; eexists; repeat split; auto.
+        apply: run_cut X H1.
+      move=> //=.
+    + move=> s1 r A B C n ++ rB IH s2 A1 B1 A2 B2 ???; subst.
+      move=> /=; case: ifP => [dA fB|dA fA].
+        case X: next_alt => //[B1'][?]; subst.
+        have {IH}[n1] := IH _ _ _ _ _ erefl erefl erefl.
+        case: r {rB} => //.
+        move=> [H1 [H2[H3 H4]]]; subst.
+        case: n1 H1 H2 => //=[|n1] H1.
+          move=> [n2 H]; repeat eexists; eauto.
+          move=> /=; eexists; apply: run_fail fB X H.
+        by have [_[??]] := run_dead1 _ dA H1; subst.
+      case nA1 : next_alt => [A1'|]//.
+        move=> [?]; subst.
+        have {IH}[n1] := IH _ _ _ _ _ erefl erefl erefl.
+        case: r {rB} => //.
+        move=> [H1 [H2[H3 H4]]]; subst.
+        case: n1 H1 H2 => //=[|n1] H1.
+          move=> [n2 H]; repeat eexists; eauto.
+            apply: run_fail fA nA1 H1.
+          by eexists; eauto.
+        move=> ?; subst; repeat eexists => //.
+          apply: run_fail fA nA1 H1.
+        by [].
+      case:ifP => //dB1.
+      case nB1: next_alt => [nB1'|]//=[?]; subst.
+      have {IH}[n1] := IH _ _ _ _ _ erefl erefl erefl.
+      case: r {rB} => //.
+      move=> [H1 [H2[H3 H4]]]; subst.
+      case: n1 H1 H2 => //=[|n1] H1.
+        have [_[? _]]:= run_dead2 _ H1; subst.
+        move=> [n2 H]; repeat eexists; eauto.
+          apply: run_dead fA nA1.
+        by eexists; apply: next_alt_runb; eauto.
+      move=> ?; subst; repeat eexists => //.
+        have [_[? _]]:= run_dead2 _ H1; subst.
+        apply: run_dead fA nA1.
+      by have [?[]]:= run_dead2 _ H1.
+    + move=> s1 B ++ s2 A1 B1 A2 B2 ? + _; subst => /=.
+      case:ifP => [dA1 fB1|dA1 fA1].
+        case nB1: next_alt => // _ [<-{A2}<-{B2}].
+        repeat eexists; rewrite?dead2//.
+          apply: run_dead (is_dead_failed dA1) _.
+          by rewrite is_dead_next_alt.
+        eexists; apply: run_dead fB1 nB1.
+      case nA1: next_alt => [A1'|]//=.
+      case:ifP => [dB1 _|dB1].
+        move=> [<-<-{A2 B2}].
+        repeat eexists; rewrite ?dead2//.
+          apply: run_dead fA1 nA1.
+        by eexists; apply: run_dead (is_dead_failed dB1) (is_dead_next_alt _ _).
+      case nB1: next_alt => // _ [<-<-{A2 B2}].
+      repeat eexists; rewrite ?dead2//.
+        apply: run_dead fA1 nA1.
+      eexists.
+      case X: (failed B1).
+        apply: run_dead X nB1.
+      by rewrite next_alt_not_failed in nB1.
   Qed.
 
-  Lemma run_or_correct_dead {s1 s2 A B}:
+  (* Lemma run_or_correct_dead {s1 s2 A B}:
     dead_run u s1 A -> dead_run u s2 B -> dead_run u s1 (Or A s2 B).
   Proof.
-    move=> HA HB sX C b H.
+    move=> HA HB C n.
     have [n[r'[]]] := run_or_complete H.
       by move=> []/HA.
     apply: HB.
-  Qed.
+  Qed. *)
 
   Lemma run_or_is_ko_left_ign_subst {A s B s2 D b2 sIgn1} sIgn2:
     is_ko A -> runb u sIgn1 (Or A s B) s2 D b2 ->
       runb u sIgn2 (Or A s B) s2 D 0.
   Proof.
     move=> H1 H2.
-    have [b1[r1 [H3 H4]]]:= run_ko_left1 H1 H2.
-    by have H5 := run_ko_left2 sIgn2 H1 H3; subst.
+    have:= runb_same_structure _ H2.
+    case: D H2 => //= A' s' B' + /eqP?; subst.
+    move=> /[dup] /runb_or0-> /(run_ko_left1 H1) [b'][H2 -> {A'}].
+    apply: run_ko_left2 H1 H2.
   Qed.
 
-  Lemma failed_cutl_runb A:
+  (* Lemma failed_cutl_runb A:
     failed (cutl A) -> forall s, dead_run u s (cutl A).
   Proof.
     elim: A => //=.
@@ -449,9 +580,9 @@ Section s.
       move=>[?]; subst; move: H1; rewrite /= sA success_failed//=.
       rewrite (next_alt_cutl_failed fB) next_alt_cutl_success//?if_same//.
       rewrite -success_cut//.
-  Qed.
+  Qed. *)
 
-  Lemma run_and_correct {s0 sn A B0 B r b}:
+  (* Lemma run_and_correct {s0 sn A B0 B r b}:
     runb u s0 (And A B0 B) sn r b ->
     (Texists sm r1 b1, runb u s0 A sm r1 b1 /\
       Texists b2 r2, ((runb u sm B sn r2 b2) + 
@@ -539,5 +670,5 @@ Section s.
         right; eexists; apply: next_alt_runb Y _.
         eauto.
       repeat eexists; right; eauto.
-  Qed.
+  Qed. *)
 End s.
